src/proofs/no_slashable_attestations/supporting_lemmas/fnc_invs_27_39.dfy
@@ -848,7 +848,7 @@ module Fnc_Invs_27_39
         }
     }   
 
-    lemma lemma_inv_monotonic_att_slashing_db_add_block_to_bn(
+    lemma lemma_concl_monotonic_att_slashing_db_add_block_to_bn(
         s: DVCState,
         block: BeaconBlock,
         s': DVCState 
@@ -858,7 +858,7 @@ module Fnc_Invs_27_39
     ensures s.attestation_slashing_db <= s'.attestation_slashing_db
     { }
 
-    lemma lemma_inv_monotonic_att_slashing_db_f_listen_for_attestation_shares(
+    lemma lemma_concl_monotonic_att_slashing_db_f_listen_for_attestation_shares(
         process: DVCState,
         attestation_share: AttestationShare,
         process': DVCState
@@ -868,13 +868,13 @@ module Fnc_Invs_27_39
     ensures process.attestation_slashing_db <= process'.attestation_slashing_db    
     { }
 
-    lemma lemma_inv_monotonic_att_slashing_db_f_start_next_duty(process: DVCState, attestation_duty: AttestationDuty, process': DVCState)
+    lemma lemma_concl_monotonic_att_slashing_db_f_start_next_duty(process: DVCState, attestation_duty: AttestationDuty, process': DVCState)
     requires f_start_next_duty.requires(process, attestation_duty)
     requires process' == f_start_next_duty(process, attestation_duty).state       
     ensures process.attestation_slashing_db <= process'.attestation_slashing_db 
     { } 
 
-    lemma lemma_inv_monotonic_att_slashing_db_f_resend_attestation_share(
+    lemma lemma_concl_monotonic_att_slashing_db_f_resend_attestation_share(
         process: DVCState,
         process': DVCState)
     requires f_resend_attestation_share.requires(process)
@@ -883,7 +883,7 @@ module Fnc_Invs_27_39
     { } 
 
 
-    lemma lemma_inv_monotonic_att_slashing_db_f_check_for_next_queued_duty(
+    lemma lemma_concl_monotonic_att_slashing_db_f_check_for_next_queued_duty(
         process: DVCState,
         process': DVCState
     )
@@ -914,7 +914,7 @@ module Fnc_Invs_27_39
 
                     assert process.attestation_slashing_db <= process_mod.attestation_slashing_db;
                     
-                    lemma_inv_monotonic_att_slashing_db_f_check_for_next_queued_duty(process_mod, process');
+                    lemma_concl_monotonic_att_slashing_db_f_check_for_next_queued_duty(process_mod, process');
                 }
                 else
                 { 
@@ -922,7 +922,7 @@ module Fnc_Invs_27_39
                         attestation_duties_queue := process.attestation_duties_queue[1..]
                     );     
                     assert process.attestation_slashing_db <= process_mod.attestation_slashing_db;
-                    lemma_inv_monotonic_att_slashing_db_f_start_next_duty(process_mod, process.attestation_duties_queue[0], process');
+                    lemma_concl_monotonic_att_slashing_db_f_start_next_duty(process_mod, process.attestation_duties_queue[0], process');
                 }
         }
         else
@@ -931,7 +931,7 @@ module Fnc_Invs_27_39
         }
     }
 
-    lemma lemma_inv_monotonic_att_slashing_db_f_att_consensus_decided(
+    lemma lemma_concl_monotonic_att_slashing_db_f_att_consensus_decided(
         process: DVCState,
         id: Slot,
         decided_attestation_data: AttestationData, 
@@ -974,13 +974,13 @@ module Fnc_Invs_27_39
 
             var ret_dvc := f_check_for_next_queued_duty(process_mod).state;
             
-            lemma_inv_monotonic_att_slashing_db_f_check_for_next_queued_duty(process_mod, ret_dvc);
+            lemma_concl_monotonic_att_slashing_db_f_check_for_next_queued_duty(process_mod, ret_dvc);
             
             assert process' == ret_dvc;  
         }      
     }
 
-    lemma lemma_inv_monotonic_att_slashing_db_f_serve_attestation_duty(
+    lemma lemma_concl_monotonic_att_slashing_db_f_serve_attestation_duty(
         process: DVCState,
         attestation_duty: AttestationDuty,
         process': DVCState
@@ -996,10 +996,10 @@ module Fnc_Invs_27_39
 
         assert process.attestation_slashing_db <= process_mod.attestation_slashing_db;
 
-        lemma_inv_monotonic_att_slashing_db_f_check_for_next_queued_duty(process_mod, process');        
+        lemma_concl_monotonic_att_slashing_db_f_check_for_next_queued_duty(process_mod, process');        
     }
 
-    lemma lemma_inv_monotonic_att_slashing_db_f_listen_for_new_imported_blocks(
+    lemma lemma_concl_monotonic_att_slashing_db_f_listen_for_new_imported_blocks(
         process: DVCState,
         block: BeaconBlock,
         process': DVCState
@@ -1043,20 +1043,20 @@ module Fnc_Invs_27_39
 
             
 
-            lemma_inv_monotonic_att_slashing_db_f_check_for_next_queued_duty(process_mod, process');
+            lemma_concl_monotonic_att_slashing_db_f_check_for_next_queued_duty(process_mod, process');
         }
         else
         { }
     } 
 
-    lemma lemma_inv_monotonic_att_slashing_db_dv_next(
+    lemma lemma_concl_monotonic_att_slashing_db_dv_next(
         dv: DVState,
         event: DV.Event,
         dv': DVState
     ) 
     requires NextEvent.requires(dv, event, dv')    
     requires NextEvent(dv, event, dv')  
-    ensures inv_monotonic_att_slashing_db(dv, event, dv')
+    ensures concl_monotonic_att_slashing_db(dv, event, dv')
     {        
         match event 
         {
@@ -1067,18 +1067,18 @@ module Fnc_Invs_27_39
                 match nodeEvent
                 {
                     case ServeAttstationDuty(attestation_duty) =>   
-                        lemma_inv_monotonic_att_slashing_db_f_serve_attestation_duty(dvc, attestation_duty, dvc');
+                        lemma_concl_monotonic_att_slashing_db_f_serve_attestation_duty(dvc, attestation_duty, dvc');
                         
                     case AttConsensusDecided(id, decided_attestation_data) => 
-                        lemma_inv_monotonic_att_slashing_db_f_att_consensus_decided(dvc, id, decided_attestation_data, dvc');
+                        lemma_concl_monotonic_att_slashing_db_f_att_consensus_decided(dvc, id, decided_attestation_data, dvc');
                         
                     case ReceivedAttestationShare(attestation_share) =>                         
-                        lemma_inv_monotonic_att_slashing_db_f_listen_for_attestation_shares(dvc, attestation_share, dvc');
+                        lemma_concl_monotonic_att_slashing_db_f_listen_for_attestation_shares(dvc, attestation_share, dvc');
                        
                     case ImportedNewBlock(block) => 
                         var dvc_mod := add_block_to_bn(dvc, block);
-                        lemma_inv_monotonic_att_slashing_db_add_block_to_bn(dvc, block, dvc_mod);
-                        lemma_inv_monotonic_att_slashing_db_f_listen_for_new_imported_blocks(dvc_mod, block, dvc');                        
+                        lemma_concl_monotonic_att_slashing_db_add_block_to_bn(dvc, block, dvc_mod);
+                        lemma_concl_monotonic_att_slashing_db_f_listen_for_new_imported_blocks(dvc_mod, block, dvc');                        
 
                     case ResendAttestationShares =>                                                                      
 
@@ -1421,48 +1421,48 @@ module Fnc_Invs_27_39
         }
     }   
     
-    lemma lemma_inv_monotonic_att_slashing_db_hist_add_block_to_bn(
+    lemma lemma_concl_monotonic_att_slashing_db_hist_add_block_to_bn(
         s: DVCState,
         block: BeaconBlock,
         s': DVCState 
     )
     requires add_block_to_bn.requires(s, block)
     requires s' == add_block_to_bn(s, block)    
-    ensures inv_monotonic_att_slashing_db_hist_body(s, s')
+    ensures concl_monotonic_att_slashing_db_hist_body(s, s')
     { }
 
-    lemma lemma_inv_monotonic_att_slashing_db_hist_f_listen_for_attestation_shares(
+    lemma lemma_concl_monotonic_att_slashing_db_hist_f_listen_for_attestation_shares(
         process: DVCState,
         attestation_share: AttestationShare,
         process': DVCState
     )
     requires f_listen_for_attestation_shares.requires(process, attestation_share)
     requires process' == f_listen_for_attestation_shares(process, attestation_share).state        
-    ensures inv_monotonic_att_slashing_db_hist_body(process, process')
+    ensures concl_monotonic_att_slashing_db_hist_body(process, process')
     { }
 
-    lemma lemma_inv_monotonic_att_slashing_db_hist_f_start_next_duty(process: DVCState, attestation_duty: AttestationDuty, process': DVCState)
+    lemma lemma_concl_monotonic_att_slashing_db_hist_f_start_next_duty(process: DVCState, attestation_duty: AttestationDuty, process': DVCState)
     requires f_start_next_duty.requires(process, attestation_duty)
     requires process' == f_start_next_duty(process, attestation_duty).state       
-    ensures inv_monotonic_att_slashing_db_hist_body(process, process')
+    ensures concl_monotonic_att_slashing_db_hist_body(process, process')
     { } 
 
-    lemma lemma_inv_monotonic_att_slashing_db_hist_f_resend_attestation_share(
+    lemma lemma_concl_monotonic_att_slashing_db_hist_f_resend_attestation_share(
         process: DVCState,
         process': DVCState)
     requires f_resend_attestation_share.requires(process)
     requires process' == f_resend_attestation_share(process).state        
-    ensures inv_monotonic_att_slashing_db_hist_body(process, process')     
+    ensures concl_monotonic_att_slashing_db_hist_body(process, process')     
     { } 
 
 
-    lemma lemma_inv_monotonic_att_slashing_db_hist_f_check_for_next_queued_duty(
+    lemma lemma_concl_monotonic_att_slashing_db_hist_f_check_for_next_queued_duty(
         process: DVCState,
         process': DVCState
     )
     requires f_check_for_next_queued_duty.requires(process)
     requires process' == f_check_for_next_queued_duty(process).state        
-    ensures inv_monotonic_att_slashing_db_hist_body(process, process')
+    ensures concl_monotonic_att_slashing_db_hist_body(process, process')
     decreases process.attestation_duties_queue
     {
         if  && process.attestation_duties_queue != [] 
@@ -1487,7 +1487,7 @@ module Fnc_Invs_27_39
 
                     assert process.attestation_slashing_db <= process_mod.attestation_slashing_db;
                     
-                    lemma_inv_monotonic_att_slashing_db_hist_f_check_for_next_queued_duty(process_mod, process');
+                    lemma_concl_monotonic_att_slashing_db_hist_f_check_for_next_queued_duty(process_mod, process');
                 }
                 else
                 { 
@@ -1495,7 +1495,7 @@ module Fnc_Invs_27_39
                         attestation_duties_queue := process.attestation_duties_queue[1..]
                     );     
                     assert process.attestation_slashing_db <= process_mod.attestation_slashing_db;
-                    lemma_inv_monotonic_att_slashing_db_hist_f_start_next_duty(process_mod, process.attestation_duties_queue[0], process');
+                    lemma_concl_monotonic_att_slashing_db_hist_f_start_next_duty(process_mod, process.attestation_duties_queue[0], process');
                 }
         }
         else
@@ -1504,7 +1504,7 @@ module Fnc_Invs_27_39
         }
     }
 
-    lemma lemma_inv_monotonic_att_slashing_db_hist_f_att_consensus_decided(
+    lemma lemma_concl_monotonic_att_slashing_db_hist_f_att_consensus_decided(
         process: DVCState,
         id: Slot,
         decided_attestation_data: AttestationData, 
@@ -1512,7 +1512,7 @@ module Fnc_Invs_27_39
     )
     requires f_att_consensus_decided.requires(process, id, decided_attestation_data)
     requires process' == f_att_consensus_decided(process, id, decided_attestation_data).state         
-    ensures inv_monotonic_att_slashing_db_hist_body(process, process')
+    ensures concl_monotonic_att_slashing_db_hist_body(process, process')
     {
         
         if  && process.current_attestation_duty.isPresent()
@@ -1547,20 +1547,20 @@ module Fnc_Invs_27_39
 
             var ret_dvc := f_check_for_next_queued_duty(process_mod).state;
             
-            lemma_inv_monotonic_att_slashing_db_hist_f_check_for_next_queued_duty(process_mod, ret_dvc);
+            lemma_concl_monotonic_att_slashing_db_hist_f_check_for_next_queued_duty(process_mod, ret_dvc);
             
             assert process' == ret_dvc;       
         } 
     }
 
-    lemma lemma_inv_monotonic_att_slashing_db_hist_f_serve_attestation_duty(
+    lemma lemma_concl_monotonic_att_slashing_db_hist_f_serve_attestation_duty(
         process: DVCState,
         attestation_duty: AttestationDuty,
         process': DVCState
     )  
     requires f_serve_attestation_duty.requires(process, attestation_duty)
     requires process' == f_serve_attestation_duty(process, attestation_duty).state
-    ensures inv_monotonic_att_slashing_db_hist_body(process, process')
+    ensures concl_monotonic_att_slashing_db_hist_body(process, process')
     {
         var process_mod := process.(
                 attestation_duties_queue := process.attestation_duties_queue + [attestation_duty],
@@ -1569,17 +1569,17 @@ module Fnc_Invs_27_39
 
         assert process.attestation_slashing_db <= process_mod.attestation_slashing_db;
 
-        lemma_inv_monotonic_att_slashing_db_hist_f_check_for_next_queued_duty(process_mod, process');        
+        lemma_concl_monotonic_att_slashing_db_hist_f_check_for_next_queued_duty(process_mod, process');        
     }
 
-    lemma lemma_inv_monotonic_att_slashing_db_hist_f_listen_for_new_imported_blocks(
+    lemma lemma_concl_monotonic_att_slashing_db_hist_f_listen_for_new_imported_blocks(
         process: DVCState,
         block: BeaconBlock,
         process': DVCState
     )
     requires f_listen_for_new_imported_blocks.requires(process, block)
     requires process' == f_listen_for_new_imported_blocks(process, block).state   
-    ensures inv_monotonic_att_slashing_db_hist_body(process, process')    
+    ensures concl_monotonic_att_slashing_db_hist_body(process, process')    
     {
         var new_consensus_instances_already_decided := f_listen_for_new_imported_blocks_helper_1(process, block);
 
@@ -1616,7 +1616,7 @@ module Fnc_Invs_27_39
 
             
 
-            lemma_inv_monotonic_att_slashing_db_hist_f_check_for_next_queued_duty(process_mod, process');
+            lemma_concl_monotonic_att_slashing_db_hist_f_check_for_next_queued_duty(process_mod, process');
         }
         else
         { }
